\documentclass{ximera}

\input{../../preamble.tex}

\author{Jason Miller}
\license{Creative Commons 3.0 By-bC}


\outcome{}


\begin{document}
\begin{exercise}
Determine the integral.
\[
\int_{0}^{\infty} xe^{-x} \d x
\]


We rewrite the improper integral as a limit 

\[
\int_{0}^{\infty} xe^{-x} \d x= \lim_{b \to \infty} \int_{0}^{b} xe^{-x} \d x
\]


First we determine the definite integral

\[
\int_{0}^{b} xe^{-x} \d x=\answer{ -be^{-b}-e^{-b} +1 } 
\]




\begin{exercise}
Now we need to calculate the limit as $b \to \infty$ of this expression. 

\[
\lim_{b \to \infty}  -be^{-b}-e^{-b} +1 =\answer{ 1}
\]

\begin{exercise}
So the  integral $\int_{0}^{\infty} xe^{-x} \d x=\answer{1}$

\begin{exercise}
 Hence we say that the integral 

\begin{multipleChoice}
\choice[correct]{converges}
\choice{diverges}
\end{multipleChoice}



\end{exercise}
\end{exercise}
\end{exercise}
\end{exercise}
\end{document}
